\documentclass[a4paper,12pt]{article}
\usepackage{graphicx}
\usepackage{amsmath}

\title{Assignment 1\\ Latex Report}
\author{Fuzayil Bin Afzal Mir}
\date{12/01/2021}
\begin{document}
	\maketitle
	
	
	\newpage
	\section{Exercise 2.17}
	\section{If 
	A =	\begin{pmatrix}
		-1 & 2 & 3\\
		 5 & 7 & 9\\
		-1 & 1 & 1\\		
	\end{pmatrix}
	and 
	B = \begin{pmatrix}
		-4 & 1 & -5\\
		 1 & 2 & 0\\
		 1 & 3 & 1\\		
	\end{pmatrix}\\
	then, verify that \\
	$$ 1) (A+B)' = A'+B' $$\\
	$$ 2) (A-B)' = A'-B' $$\\
	
	
	} 
	
	\subsection{Solution} \\
	$$ 1) (A+B)' = A'+B' $$\\

	
	Since it's given
	A =	\begin{pmatrix}
		-1 & 2 & 3\\
		 5 & 7 & 9\\
		-1 & 1 & 1\\		
	\end{pmatrix}
	and 
	B = \begin{pmatrix}
		-4 & 1 & -5\\
		 1 & 2 & 0\\
		 1 & 3 & 1\\		
	\end{pmatrix}\\
	\\
	therefore,\\L.H.S\\ 
	A+B =	\begin{pmatrix}
		(-1+(-4)) & (2+1) & (3+(-5))\\
		 (5+1) & (7+2) & (9+0)\\
		(-1+1) & (1+3) & (1+1)\\		
	\end{pmatrix}
	\\
	A+B =	\begin{pmatrix}
		-5 & 3 & -2\\
		 6 & 9 & 9\\
		 0 & 4 & 2\\		
	\end{pmatrix}
	
	Now,\\
	$$(A+B)'=\begin{pmatrix}
		-5 & 6 & 0\\
		 3 & 9 & 4\\
		-2 & 9 & 2\\		
	\end{pmatrix}$$
	
	Taking R.H.S
	$$A'=\begin{pmatrix}
		-1 & 5 & -1\\
		 2 & 7 & 1\\
		 3 & 9 & 1\\		
	\end{pmatrix}
	
		$$B'=\begin{pmatrix}
		-4 & 1 & 1\\
		 1 & 2 & 3\\
		-5 & 0 & 1\\		
	\end{pmatrix}\\
		\\
	$$
	$$
	$$
	$$
	\\
  $$Adding,$$A' and B'$$
  	\\
	$$
	$$
	$$
	$$
	\\
  
  
  
  
$$A'+B'=\begin{pmatrix}
		-5 & 6 & 0\\
		 3 & 9 & 4\\
		-2 & 9 & 2\\		
	\end{pmatrix}$$
	
	
	Now on comparing L.H.S and R.H.S
	we get,$$
	L.H.S=R.H.S \\

	$$ (A+B)' = A'+B' $$\\
	
	\\
\newpage	
	
	
	$$  (2) (A-B)' = A'-B' $$\\
	
	Since it's given
	A =	\begin{pmatrix}
		-1 & 2 & 3\\
		 5 & 7 & 9\\
		-1 & 1 & 1\\		
	\end{pmatrix}
	and 
	B = \begin{pmatrix}
		-4 & 1 & -5\\
		 1 & 2 & 0\\
		 1 & 3 & 1\\		
	\end{pmatrix}\\
	\\
	therefore,\\L.H.S\\ 
	A-B =	\begin{pmatrix}
		(-1-(-4)) & (2-1) & (3-(-5))\\
		 (5-1) & (7-2) & (9-0)\\
		(-1-1) & (1-3) & (1-1)\\		
	\end{pmatrix}
	\\
	$$
	$$
	$$
	$$
	\\
	A-B =	\begin{pmatrix}
		3 & 1 & 8\\
		4 & 5 & 9\\
	   -2 & -2 & 0\\		
	\end{pmatrix}
	\\
	$$
	$$
	$$
	$$
	\\
	Now,\\
	$$(A-B)'=\begin{pmatrix}
		 3 & 4 & -2 \\
		 1 & 5 & -2\\
		 8 & 9 & 0\\		
	\end{pmatrix}$$
		\\
	$$
	$$
	$$
	$$
	\\
	Taking R.H.S
	$$A'=\begin{pmatrix}
		-1 & 5 & -1\\
		 2 & 7 & 1\\
		 3 & 9 & 1\\		
	\end{pmatrix}
		\\
	$$
	$$

	\\
		$$B'=\begin{pmatrix}
		-4 & 1 & 1\\
		 1 & 2 & 3\\
		-5 & 0 & 1\\		
	\end{pmatrix}
	\\
	$$
	$$
	$$
	$$
	\\


\\
$$Now Subtracting B' from A' \\
	\\
	$$
	$$
	
	\\



$$Hence, A'- B'=
\begin{pmatrix}
		--1-(-4) & 5-1 & -1-1\\
		 2-1 & 7-2 & 1-3\\
		(3-(-5)) & 9-0 & 1-1\\		
	\end{pmatrix}$$
	
	\\
		\\
	$$
	$$
	\\
	$$A'-B'=
	\begin{pmatrix}
		3 & 4 & -2\\
		1 & 5 & -2\\
		8 & 9 & 0\\		
	\end{pmatrix}
	
	
	Now on comparing L.H.S and R.H.S
	we get,$$
	L.H.S=R.H.S \\

	$$ (A-B)' = A'-B' $$\\
	
\end{document}